lib/compcert-2.4/lib/Maps.v
@@ -1542,5 +1542,5 @@ Module PTree_Properties := Tree_Properties(PTree).
 
 (** * Useful notations *)
 
-Notation "a ! b" := (PTree.get b a) (at level 1).
-Notation "a !! b" := (PMap.get b a) (at level 1).
+Notation "a ? b" := (PTree.get b a) (at level 1).
+Notation "a ?? b" := (PMap.get b a) (at level 1).
