src/Vellvm/analysis.v
@@ -8,11 +8,12 @@ Require Import Memory.
 Require Import Integers.
 Require Import Coqlib.
 Require Import Maps.
+Require Import maps_ext.
 Require Import Lattice.
 Require Import Iteration.
-Require Import Kildall.
 Require Import ListSet.
 Require Import dom_list.
+Require Import util. (* for NodeSet *)
 
 (**********************************)
 (* This file defines analysis used by Vellvm. *)
