src/Vellvm/opsem_inst.v
@@ -21,6 +21,7 @@ Require Import targetdata.
 Require Import Floats.
 Require Import AST.
 Require Import Maps.
+Require Import maps_ext.
 Require Import opsem.
 Require Import opsem_props.
 Require Import opsem_wf.
